vale/code/arch/x64/X64.BufferViewStore.fsti
@@ -1,0 +1,43 @@
+module X64.BufferViewStore
+
+open Views
+open Interop
+module B = LowStar.Buffer
+module BV = LowStar.BufferView
+module HS = FStar.HyperStack
+open BufferViewHelpers
+
+open X64.Machine_s
+open X64.Bytes_Semantics_s
+
+val bv_upd_update_heap64:
+  (b:s8{B.length b % 8 == 0}) ->
+  (heap:heap) ->
+  (i:nat{i < B.length b / 8}) ->
+  (v:nat64) ->
+  (addrs:addr_map) ->
+  (ptrs:list s8) ->
+  (h:HS.mem{B.live h b}) ->
+   Lemma (
+     let bv = BV.mk_buffer_view b view64 in
+     BV.as_buffer_mk_buffer_view b view64;
+     BV.get_view_mk_buffer_view b view64;
+     BV.length_eq bv;
+     let heap' = update_heap64 (addrs b + 8 `op_Multiply` i) v heap in
+     BV.upd h bv i (UInt64.uint_to_t v) == B.g_upd_seq b (get_seq_heap heap' addrs b) h)
+
+val bv_upd_update_heap128:
+  (b:s8{B.length b % 16 == 0}) ->
+  (heap:heap) ->
+  (i:nat{i < B.length b / 16}) ->
+  (v:quad32) ->
+  (addrs:addr_map) ->
+  (ptrs:list s8) ->
+  (h:HS.mem{B.live h b}) ->
+   Lemma (
+     let bv = BV.mk_buffer_view b view128 in
+     BV.as_buffer_mk_buffer_view b view128;
+     BV.get_view_mk_buffer_view b view128;
+     BV.length_eq bv;
+     let heap' = update_heap128 (addrs b + 16 `op_Multiply` i) v heap in
+     BV.upd h bv i v == B.g_upd_seq b (get_seq_heap heap' addrs b) h)
